No need to call flushall() in [dsync] / [dsync_vecs]
Even if there are pending transactions writing to an address,
we are still safe to dsync that address. (most likely when we
first call dwrite() on that address, flushall() will be called).
This change further simplifies top-level file_sync_ok spec,
as there is no branches in its post condition.

In terms of spec and proof, the dssync/dssync_vecs operators are
commutative with replay_disk -- this is not true for dsupd, so
we might need to call flushall in dwrite().

src/GroupLog.v
@@ -238,11 +238,6 @@ Module GLog.
     mm' <- MLog.dwrite xp a v mm;
     rx (mk_memstate vm ts mm').
 
-  Definition dsync' T xp a ms rx : prog T :=
-    let '(vm, ts, mm) := (MSVMap (fst ms), MSTxns (fst ms), MSLL ms) in
-    mm' <- MLog.dsync xp a mm;
-    rx (mk_memstate vm ts mm').
-
   Definition dwrite T (xp : log_xparams) a v ms rx : prog T :=
     let '(vm, ts, mm) := (MSVMap (fst ms), MSTxns (fst ms), MSLL ms) in
     If (MapFacts.In_dec vm a) {
@@ -254,25 +249,9 @@ Module GLog.
       rx ms
     }.
 
-  Definition dsync T (xp : log_xparams) a ms rx : prog T :=
-    let '(vm, ts, mm) := (MSVMap (fst ms), MSTxns (fst ms), MSLL ms) in
-    If (MapFacts.In_dec vm a) {
-      ms <- flushall xp ms;
-      ms <- dsync' xp a ms;
-      rx ms
-    } else {
-      ms <- dsync' xp a ms;
-      rx ms
-    }.
-
   Definition dwrite_vecs' T (xp : log_xparams) avs ms rx : prog T :=
     let '(vm, ts, mm) := (MSVMap (fst ms), MSTxns (fst ms), MSLL ms) in
     mm' <- MLog.dwrite_vecs xp avs mm;
-    rx (mk_memstate vm ts mm').
-
-  Definition dsync_vecs' T xp al ms rx : prog T :=
-    let '(vm, ts, mm) := (MSVMap (fst ms), MSTxns (fst ms), MSLL ms) in
-    mm' <- MLog.dsync_vecs xp al mm;
     rx (mk_memstate vm ts mm').
 
   Definition dwrite_vecs T (xp : log_xparams) avs ms rx : prog T :=
@@ -286,16 +265,15 @@ Module GLog.
       rx ms
     }.
 
-  Definition dsync_vecs T (xp : log_xparams) al ms rx : prog T :=
+  Definition dsync T xp a ms rx : prog T :=
     let '(vm, ts, mm) := (MSVMap (fst ms), MSTxns (fst ms), MSLL ms) in
-    If (bool_dec (overlap al vm) true) {
-      ms <- flushall xp ms;
-      ms <- dsync_vecs' xp al ms;
-      rx ms
-    } else {
-      ms <- dsync_vecs' xp al ms;
-      rx ms
-    }.
+    mm' <- MLog.dsync xp a mm;
+    rx (mk_memstate vm ts mm').
+
+  Definition dsync_vecs T xp al ms rx : prog T :=
+    let '(vm, ts, mm) := (MSVMap (fst ms), MSTxns (fst ms), MSLL ms) in
+    mm' <- MLog.dsync_vecs xp al mm;
+    rx (mk_memstate vm ts mm').
 
   Definition recover T xp cs rx : prog T :=
     mm <- MLog.recover xp cs;
@@ -933,9 +911,7 @@ Module GLog.
     apply replay_seq_dssync_vecs_ents; auto.
   Qed.
 
-  Lemma dset_match_dssync_notin : forall xp ds a ts vm,
-    Map.find a vm = None ->
-    vmap_match vm ts ->
+  Lemma dset_match_dssync : forall xp ds a ts,
     dset_match xp ds ts ->
     dset_match xp (dssync ds a) ts.
   Proof.
@@ -943,7 +919,6 @@ Module GLog.
     eapply forall_ents_valid_length_eq; try eassumption.
     apply length_updN.
     apply replay_seq_dssync_notin; auto.
-    eapply vmap_match_notin; eauto.
   Qed.
 
   Lemma cached_dsupd_latest_recover_any : forall xp ds a v ms hm ms0,
@@ -1018,30 +993,6 @@ Module GLog.
   Qed.
 
 
-  Theorem dsync'_ok: forall xp a ms,
-    {< F Fd ds vs,
-    PRE:hm
-      << F, rep: xp (Cached ds) ms hm >> *
-      [[ Map.find a (MSVMap (fst ms)) = None ]] *
-      [[[ fst ds ::: (Fd * a |-> vs) ]]]
-    POST:hm' RET:ms'
-      << F, rep: xp (Cached (dssync ds a)) ms' hm' >>
-    XCRASH:hm'
-      << F, would_recover_any: xp ds hm' -- >>
-    >} dsync' xp a ms.
-  Proof.
-    unfold dsync'; intros.
-    prestep; unfold rep; cancel.
-    prestep; unfold rep; cancel.
-    eapply dset_match_dssync_notin; eauto.
-
-    (* crashes *)
-    xcrash.
-    rewrite MLog.synced_recover_before.
-    rewrite recover_before_any_fst; eauto.
-  Qed.
-
-  Hint Extern 1 ({{_}} progseq (dsync' _ _ _) _) => apply dsync'_ok : prog.
   Hint Extern 1 ({{_}} progseq (dwrite' _ _ _ _) _) => apply dwrite'_ok : prog.
 
   Theorem dwrite_ok: forall xp a v ms,
@@ -1121,36 +1072,25 @@ Module GLog.
     PRE:hm
       << F, rep: xp (Cached ds) ms hm >> *
       [[[ ds !! ::: (Fd * a |-> vs) ]]]
-    POST:hm' RET:ms' exists ds',
-      << F, rep: xp (Cached (dssync ds' a)) ms' hm' >> *
-      [[ ds' = ds \/ ds' = (ds!!, nil) ]]
+    POST:hm' RET:ms'
+      << F, rep: xp (Cached (dssync ds a)) ms' hm' >>
     XCRASH:hm'
       << F, would_recover_any: xp ds hm' -- >>
     >} dsync xp a ms.
   Proof.
-    unfold dsync, rep.
-    step.
+    unfold dsync.
     prestep; unfold rep; cancel.
-    prestep; unfold rep; cancel.
+    eapply list2nmem_ptsto_cancel_pair.
+    eapply diskset_ptsto_bound_latest; eauto.
 
-    erewrite fst_pair by reflexivity.
-    cancel.
-    eauto.
-    substl (MSVMap a0); eauto.
-    simpl; pred_apply; cancel.
-    step.
+    prestep; unfold rep; cancel.
+    eapply dset_match_dssync; eauto.
 
     cancel.
     repeat xcrash_rewrite; xform_norm.
     cancel; xform_normr; cancel.
-    eapply recover_latest_any; eauto.
-
-    prestep; unfold rep; cancel.
-    apply MapFacts.not_find_in_iff; auto.
-    eapply list2nmem_ptsto_cancel_pair.
-    eapply diskset_ptsto_bound_latest; eauto.
-
-    step.
+    rewrite MLog.synced_recover_before.
+    rewrite recover_before_any_fst; eauto.
     Unshelve. eauto.
   Qed.
 
@@ -1180,19 +1120,6 @@ Module GLog.
     eapply forall_ents_valid_length_eq; try eassumption.
     apply vsupd_vecs_length.
     apply replay_seq_dsupd_vecs_disjoint; auto.
-    eapply vmap_match_nonoverlap; eauto.
-  Qed.
-
-  Lemma dset_match_dssync_vecs_nonoverlap : forall xp al vm ds ts,
-    overlap al vm = false ->
-    vmap_match vm ts ->
-    dset_match xp ds ts ->
-    dset_match xp (dssync_vecs ds al) ts.
-  Proof.
-    unfold dset_match; intuition; simpl in *.
-    eapply forall_ents_valid_length_eq; try eassumption.
-    apply vssync_vecs_length.
-    apply replay_seq_dssync_vecs_disjoint; auto.
     eapply vmap_match_nonoverlap; eauto.
   Qed.
 
@@ -1226,30 +1153,7 @@ Module GLog.
     all: simpl; eauto.
   Qed.
 
-  Theorem dsync_vecs'_ok: forall xp al ms,
-    {< F ds,
-    PRE:hm
-      << F, rep: xp (Cached ds) ms hm >> *
-      [[ overlap al (MSVMap (fst ms)) = false ]] *
-      [[ Forall (fun e => e < length (fst ds)) al ]]
-    POST:hm' RET:ms'
-      << F, rep: xp (Cached (dssync_vecs ds al)) ms' hm' >>
-    XCRASH:hm'
-      << F, would_recover_any: xp ds hm' -- >>
-    >} dsync_vecs' xp al ms.
-  Proof.
-    unfold dsync_vecs'.
-    prestep; unfold rep; cancel.
-    prestep; unfold rep; cancel.
-    eapply dset_match_dssync_vecs_nonoverlap; eauto.
-
-    xcrash.
-    rewrite MLog.synced_recover_before.
-    eapply recover_before_any_fst; eauto.
-  Qed.
-
   Hint Extern 1 ({{_}} progseq (dwrite_vecs' _ _ _) _) => apply dwrite_vecs'_ok : prog.
-  Hint Extern 1 ({{_}} progseq (dsync_vecs' _ _ _) _) => apply dsync_vecs'_ok : prog.
 
   Theorem dwrite_vecs_ok: forall xp avl ms,
     {< F ds,
@@ -1318,39 +1222,27 @@ Module GLog.
     PRE:hm
       << F, rep: xp (Cached ds) ms hm >> *
       [[ Forall (fun e => e < length (ds!!)) al ]]
-    POST:hm' RET:ms' exists ds',
-      << F, rep: xp (Cached (dssync_vecs ds' al)) ms' hm' >> *
-      [[ ds' = ds \/ ds' = (ds!!, nil) ]]
+    POST:hm' RET:ms'
+      << F, rep: xp (Cached (dssync_vecs ds al)) ms' hm' >>
     XCRASH:hm'
       << F, would_recover_any: xp ds hm' -- >>
     >} dsync_vecs xp al ms.
   Proof.
-    unfold dsync_vecs, rep.
-    step.
+    unfold dsync_vecs.
     prestep; unfold rep; cancel.
-    prestep; unfold rep; cancel.
-
-    erewrite fst_pair by reflexivity.
-    cancel.
-    eauto.
-    substl (MSVMap a).
-    apply overlap_empty; apply map_empty_vmap0.
-    eauto.
-
-    step.
-    cancel.
-    repeat xcrash_rewrite; xform_norm.
-    cancel; xform_normr; cancel.
-    eapply recover_latest_any; eauto.
-
-    prestep; unfold rep; cancel.
-    apply not_true_is_false; auto.
     rewrite Forall_forall in *; intros.
     erewrite <- replay_seq_latest_length; eauto.
     unfold dset_match in *; intuition eauto.
-    step.
-  Qed.
 
+    prestep; unfold rep; cancel.
+    eapply dset_match_dssync_vecs; eauto.
+
+    cancel.
+    repeat xcrash_rewrite; xform_norm.
+    cancel; xform_normr; cancel.
+    rewrite MLog.synced_recover_before.
+    rewrite recover_before_any_fst; eauto.
+  Qed.
 
   Definition recover_any_pred xp ds hm :=
     ( exists d n ms, [[ n <= length (snd ds) ]] *
